src/Examples/Interval/CallString/Example_Interval_DG_CallString_K1.thy
@@ -567,7 +567,7 @@ definition nest_1_graph_config ::
       cluster_label = (\<lambda>owner ctx.
         if owner = ''main'' \<and> ctx = [] then ''main / root context''
         else owner @ '' / call string='' @ ''['' @ join_source '', '' (map string_of_cfg_node ctx) @ '']''),
-      source_text = Some (pretty_string_of_program nest_pi nest_procs nest_main),
+      source_text = Some (pretty_string_of_program nest_pi nest_procs nest_main []),
       node_annotation = (\<lambda>_. None)
     \<rparr>"
 
