src/Examples/Parity/Example_Parity_DG_Flagship.thy
@@ -297,7 +297,7 @@ definition parity_graph_config ::
       show_internal_globals = True,
       owner_of = (\<lambda>_. ''main''),
       cluster_label = (\<lambda>_ _. ''main / root context''),
-      source_text = Some (pretty_string_of_program parity_pi [] parity_prog),
+      source_text = Some (pretty_string_of_program parity_pi [] parity_prog []),
       node_annotation = (\<lambda>_. None)
     \<rparr>"
 
